Setlec/Verify/InferLeaves.lean
@@ -739,7 +739,7 @@ theorem inferTypeCore_WScoped {env : Env} (henv : EnvWF env) :
       simp only [WScoped]
       exact ⟨hw.1, WScoped.abstract1 0 hwbt⟩
     | app f a =>
-      obtain ⟨tf, n', ty', body', m', ta, htf, hwh, -, -, rfl⟩ :=
+      obtain ⟨tf, n', ty', body', m', htf, hwh, rfl, -⟩ :=
         inferTypeCore_app_inv h
       simp only [WScoped] at hw
       have hwtf := inferTypeCore_WScoped henv fuel htf hw.1
@@ -872,7 +872,7 @@ theorem inferTypeCore_fvarLeaves {env : Env} (henv : EnvWF env) :
           · exact absurd rfl hlne
           · exact Or.inl hb
     | app f a =>
-      obtain ⟨tf, n', ty', body', m', ta, htf, hwh, -, -, rfl⟩ :=
+      obtain ⟨tf, n', ty', body', m', htf, hwh, rfl, -⟩ :=
         inferTypeCore_app_inv h
       simp only [WScoped] at hw
       intro l hl
@@ -1008,7 +1008,7 @@ theorem inferTypeCore_looseBVars {env : Env} (henv : EnvWF env) :
       simp only [looseBVarsBounded, Bool.and_eq_true]
       exact ⟨hb.1, looseBVarsBounded_abstract1 bt 0 hbbt⟩
     | app f a =>
-      obtain ⟨tf, n', ty', body', m', ta, htf, hwh, -, -, rfl⟩ :=
+      obtain ⟨tf, n', ty', body', m', htf, hwh, rfl, -⟩ :=
         inferTypeCore_app_inv h
       simp only [WScoped] at hw
       simp only [looseBVarsBounded, Bool.and_eq_true] at hb
